src/Polara/Codegeneration/Python/Codegeneration.lean
@@ -1,6 +1,6 @@
 import Polara.Codegeneration.Utils
 
-def Const0.tmgenPy: Const0 α → String := Const0.pretty
+def Const0.tmgenPy: Const0 α → String := Const0.toString
 
 def Const1.tmgenPy (a: String): Const1 α₁ α → String
   | normCdf => "normCdf"        ++ s!"({a})"
@@ -15,9 +15,10 @@ def Const1.tmgenPy (a: String): Const1 α₁ α → String
   | suml => "sum"                ++ s!"({a})"
 
 def Const2.tmgenPy (a: String) (b: String): Const2 α₁ α₂ α → String
-  | arithOp op => s!"{a} {op.pretty} {b}"
-  | linOp op => s!"{a} {op.pretty} {b}"
-  | linScale op => s!"{a} {op.pretty} {b}"
+  | arithOp op => s!"{a} {op} {b}"
+  | linOp op => s!"{a} {op} {b}"
+  | linScale op => s!"{a} {op} {b}"
+  | lt => s!"{a} < {b}"
   | maxf => s!"max({a}, {b})"
   | addi => s!"{a} + {b}"
   | tup  => s!"({a}, {b})"
@@ -25,7 +26,7 @@ def Const2.tmgenPy (a: String) (b: String): Const2 α₁ α₂ α → String
   | get  => s!"{a}[{b}]"
 
 def Tm.codegenPy' : Tm VPar α → ReaderM (Nat × Nat) String
-  | var i => return i.pretty
+  | var i => return i.toString
   | err => return "None"
   | cst0 k => return k.tmgenPy
   | cst1 k a => return k.tmgenPy s!"({(← a.codegenPy')})"
@@ -33,15 +34,15 @@ def Tm.codegenPy' : Tm VPar α → ReaderM (Nat × Nat) String
   | abs f => do
     let (i,j) <- read
     let v := VPar.p (.mk j)
-    return s!"(lambda {v.pretty}: {(f v).codegenPy' (i,j+1)})"
+    return s!"(lambda {v}: {(f v).codegenPy' (i,j+1)})"
   | bld (n:=n) f => do
     let (i,j) <- read
     let v := VPar.p (.mk j)
-    return s!"[{(f v).codegenPy' (i,j+1)} for {v.pretty} in range(0,{n})]"
+    return s!"[{(f v).codegenPy' (i,j+1)} for {v} in range(0,{n})]"
   | bnd e f => do
     let (i,j) <- read
     let x := VPar.v (.mk i)
-    return s!"let({x.pretty} := {e.codegenPy' (i,j)}, {(f x).codegenPy' (i+1,j)})"
+    return s!"let({x} := {e.codegenPy' (i,j)}, {(f x).codegenPy' (i+1,j)})"
   | ite cond a b =>
     return s!"({<- a.codegenPy'} if {<- cond.codegenPy'} else {<- b.codegenPy'})"
 
