src/Polara/Optimizations/LinearityErasure.lean
@@ -1,0 +1,87 @@
+import Polara.Syntax.Index
+
+-- linearity erasure
+-- linErase
+@[reducible]
+def Ty.le: Ty → Ty :=
+  Ty.map (λ
+  | .lin => .flt
+  | α => α)
+def Const0.le: Const0 α → Const0 α.le
+| .litl l => .litf l
+| .litn n => .litn n
+| .litf f => .litf f
+| .liti i => .liti i
+| .litu => .litu
+| .litr => .litr
+def Const1.le: Const1 α β → Const1 α.le β.le
+| .suml => .sumf
+| .exp => .exp
+| .sqrt => .sqrt
+| .log => .log
+| .normCdf => .normCdf
+| .fst => .fst
+| .snd => .snd
+| .sumf => .sumf
+| .i2n => .i2n
+| .n2f => .n2f
+def Const2.le: Const2 α β γ → Const2 α.le β.le γ.le
+| linOp (type:=t) op =>
+  have: BiArraysC BiArith α.le β.le γ.le := ⟨
+    let rec goO {α β γ: Ty}: BiArrays BiLin α β γ → BiArrays BiArith α.le β.le γ.le
+    | .array n t' => .array n (goO t')
+    | .base t' => .base (match t' with | .lins => .flts)
+    goO t.t⟩
+  (.arithOp op.toArith)
+| linScale (type:=t) op =>
+  have: BiArraysC BiArith α.le β.le γ.le := ⟨
+    let goS {α β γ: Ty}: BiLF α β γ → BiArith α.le β.le γ.le := λ | .lf => .flts
+    match t.t with
+    | .array n t' => .array n (.base (goS t'))
+    | .base t' => .base (goS t')
+  ⟩
+  (.arithOp op.toArith)
+| .arithOp (type:=t) op =>
+  have: BiArraysC BiArith α.le β.le γ.le := ⟨
+    let rec goA {α β γ: Ty}: BiArrays BiArith α β γ → BiArrays BiArith α.le β.le γ.le
+    | .array n t' => .array n (goA t')
+    | .base t' => .base (match t' with | .nats => .nats | .flts => .flts)
+    goA t.t⟩
+  (.arithOp op)
+| .addi => .addi
+| .maxf => maxf
+| .lt => .lt
+| .get => .get
+| .tup => .tup
+| .app => .app
+def Tm.le : Tm VPar α → Tm VPar α.le
+| .err => .err
+| .cst0 const0 => Tm.cst0 const0.le
+| .cst1 const1 t => Tm.cst1 const1.le t.le
+| .cst2 const2 a b => Tm.cst2 const2.le a.le b.le
+| .abs f => .abs (λ x => (f x.changeType).le)
+| .bld a => .bld (λ idx => (a idx).le)
+| .ite cond a b => .ite cond.le a.le b.le
+| .var v => .var v.changeType
+| .bnd rest l => .bnd rest.le (λ v => (l v.changeType).le)
+| .ref (α:=α) f => .ref (λ (x: VPar α.le) xr => (f x.changeType xr.changeType).le)
+| .bndRef xr x => .bndRef xr.le x.le
+def AINF.le: AINF α → AINF α.le
+| (bnds, ret) => (bnds.map (λ ⟨⟨α,v⟩,env,prim⟩ =>
+  ⟨⟨α.le,v.changeType⟩,env.map (λ
+  | .func α x => .func α.le x.changeType
+  | .forc n i => .forc n i -- idx does not change
+  | .itec i b => .itec i b -- nat does not change
+  ),match prim with
+  | .cst0 const0 => .cst0 const0.le
+  | .cst1 const1 t => .cst1 const1.le t.changeType
+  | .cst2 const2 a b => .cst2 const2.le a.changeType b.changeType
+  | .err => .err
+  | .var v => .var v.changeType
+  | .abs x y => .abs x.changeType y.changeType
+  | .bld i x => .bld i x.changeType
+  | .ite cond a b => .ite cond.changeType a.changeType b.changeType
+  | .ref x => .ref x.changeType
+  | .bndRef (α:=α) xr x => .bndRef (α:=α.le) xr.changeType x.changeType
+  ⟩
+), ret.changeType)
