src/Polara/Optimizations/ToTm.lean
@@ -3,11 +3,13 @@ import Polara.Optimizations.CSE
 
 -- variable type in target language needs to consider environment
 @[reducible]
-def Env.tygenTm (t: Ty) (env: Env): Ty := match env with
-  | .nil => t
-  | .func env α _i  => env.tygenTm (α ~> t)
-  | .forc env n _i  => env.tygenTm (Ty.array n t)
-  | .itec env _i _m => env.tygenTm t
+def EnvPart.tygenTm (t: Ty) (env: EnvPart): Ty := match env with
+  | .func α _i  => (α ~> t)
+  | .forc n _i  => (Ty.array n t)
+  | .itec _i _m => t
+
+def Env.tygenTm (env: Env): Ty → Ty :=
+  env.foldl EnvPart.tygenTm
 
 def RenParTm (Γ: Ty → Type) := ListMap Par Γ
 def RenParTm.apply (ren: RenParTm Γ) (x: Par α): Tm Γ α :=
@@ -28,12 +30,12 @@ def RenTm.addVar (ren: RenTm Γ) (x: Var α) (y: EnvVar Γ α): RenTm Γ :=
 
 def Env.withargsTm (env: Env)(ren: RenParTm Γ)(x: Tm Γ (env.tygenTm α)): Tm Γ α :=
   match env with
-  | .nil           => x
-  | .func env' _α i  =>
-      Tm.cst2 Const2.app (env'.withargsTm ren x) (ren.apply i)
-  | .forc env' _n i  =>
-      Tm.cst2 Const2.get (env'.withargsTm ren x) (ren.apply i)
-  | .itec env' _i _b => env'.withargsTm ren x
+  | []           => x
+  | .func _α i :: env' =>
+      Tm.cst2 Const2.app (Env.withargsTm env' ren x) (ren.apply i)
+  | .forc _n i :: env' =>
+      Tm.cst2 Const2.get (Env.withargsTm env' ren x) (ren.apply i)
+  | .itec _i _b :: env' => Env.withargsTm env' ren x
 
 def RenTm.apply (ren: RenTm Γ) (x: VPar α): Tm Γ α :=
   match x with
@@ -61,39 +63,39 @@ def Prim.toTm (_env: Env)(ren: RenTm Γ): Prim α → Tm Γ α
 -- wrap environment around term depending on done renamings
 def Env.wrapTm (ren: RenTm Γ)(k: RenTm Γ → Tm Γ α)(env: Env): (Tm Γ (env.tygenTm α)) :=
   match env with
-  | .nil => k ren
-  | .func env _ i =>
-      env.wrapTm ren (λ ren => fun'v i' =>
+  | [] => k ren
+  | .func _ i :: env =>
+      Env.wrapTm ren (λ ren => fun'v i' =>
         let ren' := ren.addPar i i'
         k ren'
-      )
-  | .forc env _ i =>
-      env.wrapTm ren (λ ren => for'v i' =>
+      ) env
+  | .forc _ i :: env =>
+      Env.wrapTm ren (λ ren => for'v i' =>
         let ren' := ren.addPar i i'
         k ren'
-      )
-  | .itec env cond true  =>
-      env.wrapTm ren (λ ren =>
+      ) env
+  | .itec cond true :: env =>
+      Env.wrapTm ren (λ ren =>
         let cond' := ren.apply cond
         if' cond' then k ren else Tm.err -- undefined instead?
-      )
-  | .itec env cond false =>
-      env.wrapTm ren (λ ren =>
+      ) env
+  | .itec cond false :: env =>
+      Env.wrapTm ren (λ ren =>
         let cond' := ren.apply cond
         if' cond' then Tm.err else k ren -- undefined instead?
-      )
+      ) env
 
 -- todo zeta reduction for env to prim
 def AINF.toTm'(a: AINF α)(ren: RenTm Γ): Tm Γ α :=
   match a with
-  | .ret v => match v with
+  | ([], v) => match v with
     | .v v => match ren.var.lookup v with
       | some ⟨.nil, x'⟩ => Tm.var x'
       | _               => Tm.err
     | .p p => ren.par.apply p
-  | .bnd env v prim rest =>
+  | (⟨⟨_,v⟩, env, prim⟩ :: rest, ret) =>
     let'v v' := env.wrapTm ren (λ ren' => prim.toTm env ren');
-    rest.toTm' (ren.addVar v ⟨env, v'⟩)
+    AINF.toTm' (rest, ret) (ren.addVar v ⟨env, v'⟩)
 
 def AINF.toTm (a: AINF α): Tm Γ α := a.toTm' ⟨[], []⟩
 
