src/Polara/Tests/TestCases/Ainf.lean
@@ -7,195 +7,202 @@ namespace AinfTestCases
 
   def ainfSimpleTestCases : List (TestCase (Some AINF)) := [
     -- cst0
-    ⟨"litn", Ty.nat,
-        let'' [] in x0 := plitn 42;
-        .ret (.v x0)
+    ⟨"litn", Ty.nat, ([
+            let'' [] in x0 := plitn 42
+        ], .v x0)
     ⟩,
-    ⟨"litf", Ty.flt,
-        let'' [] in x0 := plitf 4.2;
-        .ret (.v x0)
+    ⟨"litf", Ty.flt, ([
+            let'' [] in x0 := plitf 4.2
+        ], .(.v x0))
     ⟩,
-    ⟨"liti", idx 5,
-        let'' [] in (x0: Var (idx 5)) := Prim.cst0 (liti (2: Fin 6));
-        .ret (.v x0)
+    ⟨"liti", idx 5, ([
+            let'' [] in (x0: Var (idx 5)) := Prim.cst0 (liti (2: Fin 6))
+        ], .v x0)
     ⟩,
     -- cst1
-    ⟨"exp", flt,
-        let'' [] in x0 := plitf 4.2;
-        let'' [] in x1 := cst1 exp (.v x0);
-        .ret (.v x1)
+    ⟨"exp", flt, ([
+            let'' [] in x0 := plitf 4.2,
+            let'' [] in x1 := cst1 exp (.v x0)
+        ], .v x1)
     ⟩,
-    ⟨"sqrt", flt,
-        let'' [] in x0 := plitf 4.2;
-        let'' [] in x1 := cst1 sqrt (.v x0);
-        .ret (.v x1)
+    ⟨"sqrt", flt, ([
+            let'' [] in x0 := plitf 4.2,
+            let'' [] in x1 := cst1 sqrt (.v x0)
+        ], .v x1)
     ⟩,
-    ⟨"log", flt,
-        let'' [] in x0 := plitf 4.2;
-        let'' [] in x1 := cst1 log (.v x0);
-        .ret (.v x1)
+    ⟨"log", flt, ([
+            let'' [] in x0 := plitf 4.2,
+            let'' [] in x1 := cst1 log (.v x0)
+        ], .v x1)
     ⟩,
-    ⟨"normCdf", flt,
-        let'' [] in x0 := plitf 4.2;
-        let'' [] in x1 := cst1 normCdf (.v x0);
-        .ret (.v x1)
+    ⟨"normCdf", flt, ([
+            let'' [] in x0 := plitf 4.2,
+            let'' [] in x1 := cst1 normCdf (.v x0)
+        ], .v x1)
     ⟩,
     ⟨"fst", flt,
         let x0: Var _ := (Var.mk 0)
         let x1: Var _ := x1
         let x2: Var _ := x2
         let x3: Var _ := x3
-        let'' [] in x0 := plitf 4.2;
-        let'' [] in x1 := plitn 42;
-        let'' [] in x2 := cst2 tup (.v x0) (.v x1);
-        let'' [] in x3 := cst1 fst (.v x2);
-        .ret (.v x3)
+        ([
+            let'' [] in x0 := plitf 4.2,
+            let'' [] in x1 := plitn 42,
+            let'' [] in x2 := cst2 tup (.v x0) (.v x1),
+            let'' [] in x3 := cst1 fst (.v x2)
+        ], .v x3)
     ⟩,
-    ⟨"snd", nat,
-        let'' [] in x0 := plitf 4.2;
-        let'' [] in x1 := plitn 42;
-        let'' [] in x2 := cst2 tup (.v (@x0 flt)) (.v (@x1 nat));
-        let'' [] in x3 := cst1 snd (.v (x2: Var (flt ×× nat)));
-        .ret (.v x3)
+    ⟨"snd", nat, ([
+            let'' [] in x0 := plitf 4.2,
+            let'' [] in x1 := plitn 42,
+            let'' [] in x2 := cst2 tup (.v (@x0 flt)) (.v (@x1 nat)),
+            let'' [] in x3 := cst1 snd (.v (x2: Var (flt ×× nat)))
+        ], .v x3)
     ⟩,
-    ⟨"sum", flt,
-        let'' [] in x0 := plitf 42;
-        let'' [] in x1 := for'' i0:10, (.v (x0: Var flt));
-        let'' [] in x2 := cst1 sumf (.v (x1: Var (array 10 flt)));
-        .ret (.v x2)
+    ⟨"sum", flt, ([
+            let'' [] in x0 := plitf 42,
+            let'' [] in x1 := for'' i0:10, (.v (x0: Var flt)),
+            let'' [] in x2 := cst1 sumf (.v (x1: Var (array 10 flt)))
+        ], .v x2)
     ⟩,
-    ⟨"i2n", nat,
-        let'' [] in (x0: Var (idx 5)) := Prim.cst0 (liti (2: Fin 6));
-        let'' [] in x1 := cst1 i2n (.v (x0: Var (idx 5)));
-        .ret (.v x1)
+    ⟨"i2n", nat, ([
+            let'' [] in (x0: Var (idx 5)) := Prim.cst0 (liti (2: Fin 6)),
+            let'' [] in x1 := cst1 i2n (.v (x0: Var (idx 5)))
+        ], .v x1)
     ⟩,
-    ⟨"n2f", flt,
-        let'' [] in x0 := plitn 42;
-        let'' [] in x1 := cst1 n2f (.v (x0: Var nat));
-        .ret (.v x1)
+    ⟨"n2f", flt, ([
+            let'' [] in x0 := plitn 42,
+            let'' [] in x1 := cst1 n2f (.v (x0: Var nat))
+        ], .v x1)
     ⟩,
     -- cst2
     ⟨"addn", nat,
         let x0: Var _ := (Var.mk 0)
         let x1: Var _ := x1
         let x2: Var _ := x2
-        let'' [] in x0 := plitn 42;
-        let'' [] in x1 := plitn 2;
-        let'' [] in x2 := cst2 (arithOp add) (.v x0) (.v x1);
-        .ret (.v x2)
+        ([
+            let'' [] in x0 := plitn 42,
+            let'' [] in x1 := plitn 2,
+            let'' [] in x2 := cst2 (arithOp add) (.v x0) (.v x1)
+        ], .v x2)
     ⟩,
     ⟨"muln", nat,
         let x0: Var _ := (Var.mk 0)
         let x1: Var _ := x1
         let x2: Var _ := x2
-        let'' [] in x0 := plitn 42;
-        let'' [] in x1 := plitn 2;
-        let'' [] in x2 := cst2 (arithOp mul) (.v x0) (.v x1);
-        .ret (.v x2)
+        ([
+            let'' [] in x0 := plitn 42,
+            let'' [] in x1 := plitn 2,
+            let'' [] in x2 := cst2 (arithOp mul) (.v x0) (.v x1)
+        ], .v x2)
     ⟩,
     ⟨"addf", flt,
         let x0: Var _ := (Var.mk 0)
         let x1: Var _ := x1
         let x2: Var _ := x2
-        let'' [] in x0 := plitf 42.0;
-        let'' [] in x1 := plitf 2.0;
-        let'' [] in x2 := cst2 (arithOp add) (.v x0) (.v x1);
-        .ret (.v x2)
+        ([
+            let'' [] in x0 := plitf 42.0,
+            let'' [] in x1 := plitf 2.0,
+            let'' [] in x2 := cst2 (arithOp add) (.v x0) (.v x1)
+        ], .v x2)
     ⟩,
     ⟨"subf", flt,
         let x0: Var _ := (Var.mk 0)
         let x1: Var _ := x1
         let x2: Var _ := x2
-        let'' [] in x0 := plitf 42.0;
-        let'' [] in x1 := plitf 2.0;
-        let'' [] in x2 := cst2 (arithOp sub) (.v x0) (.v x1);
-        .ret (.v x2)
+        ([
+            let'' [] in x0 := plitf 42.0,
+            let'' [] in x1 := plitf 2.0,
+            let'' [] in x2 := cst2 (arithOp sub) (.v x0) (.v x1)
+        ], .v x2)
     ⟩,
     ⟨"mulf", flt,
         let x0: Var _ := (Var.mk 0)
         let x1: Var _ := x1
         let x2: Var _ := x2
-        let'' [] in x0 := plitf 42.0;
-        let'' [] in x1 := plitf 2.0;
-        let'' [] in x2 := cst2 (arithOp mul) (.v x0) (.v x1);
-        .ret (.v x2)
+        ([
+            let'' [] in x0 := plitf 42.0,
+            let'' [] in x1 := plitf 2.0,
+            let'' [] in x2 := cst2 (arithOp mul) (.v x0) (.v x1)
+        ], .v x2)
     ⟩,
     ⟨"divf", flt,
         let x0: Var _ := (Var.mk 0)
         let x1: Var _ := x1
         let x2: Var _ := x2
-        let'' [] in x0 := plitf 42.0;
-        let'' [] in x1 := plitf 2.0;
-        let'' [] in (x2: Var flt) := cst2 (arithOp div) (.v x0) (.v x1);
-        .ret (.v x2)
+        ([
+            let'' [] in x0 := plitf 42.0,
+            let'' [] in x1 := plitf 2.0,
+            let'' [] in (x2: Var flt) := cst2 (arithOp div) (.v x0) (.v x1)
+        ], .v x2)
     ⟩,
-    ⟨"maxf", flt,
-        let'' [] in x0 := plitf 42.0;
-        let'' [] in x1 := plitf 2.0;
-        let'' [] in x2 := cst2 maxf (.v x0) (.v x1);
-        .ret (.v x2)
+    ⟨"maxf", flt, ([
+            let'' [] in x0 := plitf 42.0,
+            let'' [] in x1 := plitf 2.0,
+            let'' [] in x2 := cst2 maxf (.v x0) (.v x1)
+        ], .v x2)
     ⟩,
-    ⟨"addi", idx 10,
-        let'' [] in (x0: Var (idx 5)) := Prim.cst0 (liti (2: Fin 6));
-        let'' [] in (x1: Var (idx 5)) := Prim.cst0 (liti (2: Fin 6));
-        let'' [] in x2 := cst2 addi (.v (x0: Var (idx 5))) (.v (x1: Var (idx 5)));
-        .ret (.v x2)
+    ⟨"addi", idx 10, ([
+            let'' [] in (x0: Var (idx 5)) := Prim.cst0 (liti (2: Fin 6)),
+            let'' [] in (x1: Var (idx 5)) := Prim.cst0 (liti (2: Fin 6)),
+            let'' [] in x2 := cst2 addi (.v (x0: Var (idx 5))) (.v (x1: Var (idx 5)))
+        ], .v x2)
     ⟩,
-    ⟨"get", flt,
-        let'' [] in x0 := plitf 4.2;
-        let'' [] in x1 := for'' i0:10, (.v (x0: Var flt));
-        let'' [] in (x2: Var (idx 10)) := cst0 (liti (2: Fin 11));
-        let'' [] in x3 := cst2 get (.v (x1: Var (array 10 flt))) (.v (x2: Var (idx 10)));
-        .ret (.v x3)
+    ⟨"get", flt, ([
+            let'' [] in x0 := plitf 4.2,
+            let'' [] in x1 := for'' i0:10, (.v (x0: Var flt)),
+            let'' [] in (x2: Var (idx 10)) := cst0 (liti (2: Fin 11)),
+            let'' [] in x3 := cst2 get (.v (x1: Var (array 10 flt))) (.v (x2: Var (idx 10)))
+        ], .v x3)
     ⟩,
-    ⟨"tup", flt ×× nat,
-        let'' [] in x0 := plitf 4.2;
-        let'' [] in x1 := plitn 42;
-        let'' [] in x2 := cst2 tup (.v (x0: Var flt)) (.v (x1: Var nat));
-        .ret (.v x2)
+    ⟨"tup", flt ×× nat, ([
+            let'' [] in x0 := plitf 4.2,
+            let'' [] in x1 := plitn 42,
+            let'' [] in x2 := cst2 tup (.v (x0: Var flt)) (.v (x1: Var nat))
+        ], .v x2)
     ⟩,
-    ⟨"app", flt,
-        let'' [] in x0 := plitf 4.2;
-        let'' [] in x1 := fun'' (i0: Par nat), (.v (x0: Var flt));
-        let'' [] in (x2: Var nat) := plitn 42;
-        let'' [] in x3 := cst2 app (.v (x1: Var (nat ~> flt))) (.v (x2: Var nat));
-        .ret (.v x3)
+    ⟨"app", flt, ([
+            let'' [] in x0 := plitf 4.2,
+            let'' [] in x1 := fun'' (i0: Par nat), (.v (x0: Var flt)),
+            let'' [] in (x2: Var nat) := plitn 42,
+            let'' [] in x3 := cst2 app (.v (x1: Var (nat ~> flt))) (.v (x2: Var nat))
+        ], .v x3)
     ⟩,
     -- prim
-    ⟨"var", nat,
-        let'' [] in x0 := plitn 42;
-        let'' [] in x1 := Prim.var (.v (x0: Var nat));
-        .ret (.v x1)
+    ⟨"var", nat, ([
+            let'' [] in x0 := plitn 42,
+            let'' [] in x1 := Prim.var (.v (x0: Var nat))
+        ], .v x1)
     ⟩,
-    ⟨"abs", flt,
-        let'' [] in x0 := plitf 4.2;
-        let'' [] in x1 := fun'' (i0: Par nat), (.v (x0: Var flt));
-        -- app because function can't be printed
-        let'' [] in (x2: Var nat) := plitn 42;
-        let'' [] in x3 := cst2 app (.v (x1: Var (nat ~> flt))) (.v (x2: Var nat));
-        .ret (.v x3)
+    ⟨"abs", flt, ([
+            let'' [] in x0 := plitf 4.2,
+            let'' [] in x1 := fun'' (i0: Par nat), (.v (x0: Var flt)),
+            -- app because function can't be printed
+            let'' [] in (x2: Var nat) := plitn 42,
+            let'' [] in x3 := cst2 app (.v (x1: Var (nat ~> flt))) (.v (x2: Var nat))
+        ], .v x3)
     ⟩,
-    ⟨"bld", array 10 flt,
-        let'' [] in x0 := plitf 4.2;
-        let'' [] in x1 := for'' i0:10, (.v (x0: Var flt));
-        .ret (.v x1)
+    ⟨"bld", array 10 flt, ([
+            let'' [] in x0 := plitf 4.2,
+            let'' [] in x1 := for'' i0:10, (.v (x0: Var flt))
+        ], .v x1)
     ⟩,
-    ⟨"ite", flt,
-        let'' [] in x0 := plitn 42;
-        let'' [] in x1 := plitf 4.2;
-        let'' [] in x2 := plitf 2.4;
-        let'' [] in x3 := if'' (.v (x0: Var nat)) then (.v (x1: Var flt)) else (.v (x2: Var flt));
-        .ret (.v x3)
+    ⟨"ite", flt, ([
+            let'' [] in x0 := plitn 42,
+            let'' [] in x1 := plitf 4.2,
+            let'' [] in x2 := plitf 2.4,
+            let'' [] in x3 := if'' (.v (x0: Var nat)) then (.v (x1: Var flt)) else (.v (x2: Var flt))
+        ], .v x3)
     ⟩,
     -- more complex
-    ⟨"vectorRange", array 10 flt,
-        let'' [forc 10 i0] in x0 := cst1 i2n (.p (i0: Par (idx 10)));
-        let'' [forc 10 i0] in x1 := cst1 n2f (.v (x0: Var nat));
-        let'' [] in x2 := for'' i0:10, (.v (x1: Var flt));
-        .ret (.v x2)
-        -- let'' [forc 10 i0] in x0 := cst1 n2f (.p (i0: Par nat));
-        -- let'' [] in x1 := for'' i0:10, (.v (x0: Var flt));
-        -- .ret (.v x1)
+    ⟨"vectorRange", array 10 flt, ([
+            let'' [forc 10 i0] in x0 := cst1 i2n (.p (i0: Par (idx 10))),
+            let'' [forc 10 i0] in x1 := cst1 n2f (.v (x0: Var nat)),
+            let'' [] in x2 := for'' i0:10, (.v (x1: Var flt)),
+        ], .v x2)
+        -- let'' [forc 10 i0] in x0 := cst1 n2f (.p (i0: Par nat)),
+        -- let'' [] in x1 := for'' i0:10, (.v (x0: Var flt)),
+        -- ], .v x1)
     ⟩,
   ]
 
@@ -204,38 +211,37 @@ namespace AinfTestCases
   ------------------------------------------------------------------------------------------
   def ainfInvalidTestCases: List (TestCase (Some AINF)) := [
     ⟨"nonExistingVar", nat,
-      .ret (.v x0)
+      ([], .v x0)
     ⟩,
-    ⟨"wrongVarType", flt,
-      let'' [] in x0 := plitn 42;
-      .ret (.v x1)
+    ⟨"wrongVarType", flt, ([
+            let'' [] in x0 := plitn 42,
+      ], .v x1)
     ⟩,
-    ⟨"nonEmptyReturnEnv", array 10 flt,
-      let'' [forc 10 i0] in x0 := plitf 4.2;
-      .ret (.v x0)
+    ⟨"nonEmptyReturnEnv", array 10 flt, ([
+            let'' [forc 10 i0] in x0 := plitf 4.2,
+      ], .v x0)
     ⟩,
-    ⟨"incompatibleEnvFor", flt,
-      let'' [forc 10 i0] in x0 := plitf 4.2;
-      let'' [] in x1 := var (.v (x0: Var flt));
-      .ret (.v x1)
+    ⟨"incompatibleEnvFor", flt, ([
+      let'' [forc 10 i0] in x0 := plitf 4.2,
+      let'' [] in x1 := var (.v (x0: Var flt)),
+      ], .v x1)
     ⟩,
-    ⟨"incompatibleEnvFun", flt,
-      let'' [func nat i0] in x0 := plitf 4.2;
-      let'' [] in x1 := var (.v (x0: Var flt));
-      .ret (.v x1)
+    ⟨"incompatibleEnvFun", flt, ([
+            let'' [func nat i0] in x0 := plitf 4.2,
+            let'' [] in x1 := var (.v (x0: Var flt)),
+      ], .v x1)
     ⟩,
-    ⟨"incompatibleEnvIf", flt,
-      let'' [] in x0 := plitn 42;
-      let'' [itec (.v x0: VPar nat) true] in x1 := plitf 4.2;
-      let'' [] in x2 := var (.v (x0: Var flt));
-      .ret (.v x2)
+    ⟨"incompatibleEnvIf", flt, ([
+            let'' [] in x0 := plitn 42,
+            let'' [itec (.v x0: VPar nat) true] in x1 := plitf 4.2,
+            let'' [] in x2 := var (.v (x0: Var flt)),
+      ], .v x2)
     ⟩,
-    ⟨"multipleDefinitionsVar", flt,
-      let'' [] in x0 := plitf 4.2;
-      let'' [] in x0 := plitf 4.2;
-      .ret (.v x0)
+    ⟨"multipleDefinitionsVar", flt, ([
+            let'' [] in x0 := plitf 4.2,
+            let'' [] in x0 := plitf 4.2,
+      ], .v x0)
     ⟩,
-    -- ...
   ]
 
   def testCaseTree: TestCaseTree := Tree.node "ainf testcases"
