src/Polara/Utils/Index.lean
@@ -1,5 +1,7 @@
 import Polara.Utils.Functions
+import Polara.Utils.Graph
 import Polara.Utils.List
+import Polara.Utils.ListMap
 import Polara.Utils.Numbers
 import Polara.Utils.Option
 import Polara.Utils.Print
