src/Polara/Utils/Utils.lean
@@ -1,15 +1,26 @@
 import Polara.Utils.Print
 
--- ListMap -----------------------------------------------------------------------------------
--- List of key, value pairs, which types depend on an index Type
-def ListMap (Key Value: I → Type) := List ((index : I) × Key index × Value index)
-def ListMap.lookup [DecidableEq I][∀ x:I, BEq (K x)] : ListMap K V → K α → Option (V α)
-  | [],          _ => none
-  | ⟨β,k,v⟩::ys, i => if h: β=α then if h▸ k == i then some (h▸v)
-                      else lookup ys i else lookup ys i
-
 -----
-def Some (F: α → Type u) := (γ: α) × F γ
+abbrev Some (F: α → Type u) := (γ: α) × F γ
+def Some.of (f: F α): Some F := ⟨α, f⟩
+instance [Inhabited α][∀ γ:α, Inhabited (F γ)]: Inhabited (Some F) :=
+  ⟨Inhabited.default,Inhabited.default⟩
+instance [DecidableEq α][∀ γ, DecidableEq (F γ)]: DecidableEq (@Some α F) :=
+  λ ⟨γ,f⟩ ⟨γ',f'⟩ => if t: γ = γ' then
+    if t': t▸f=f' then
+      isTrue (by subst t; simp[t'])
+    else
+      isFalse (by subst t; simp[t'])
+  else
+    isFalse (by simp[t])
+instance [DecidableEq α][∀ γ, BEq (F γ)]: BEq (@Some α F) :=
+  ⟨λ ⟨γ,f⟩ ⟨γ',f'⟩ => if t: γ = γ' then t▸ f == f' else false⟩
+instance [Hashable α][∀ γ: α, Hashable (F γ)]: Hashable (@Some α F) :=
+  ⟨λ ⟨γ,f⟩ => mixHash (Hashable.hash γ) (Hashable.hash f)⟩
+
+instance [Inhabited α][∀ γ:α, Inhabited (F γ)]: Inhabited (Sigma F) :=
+  ⟨Inhabited.default,Inhabited.default⟩
+instance [Inhabited β]: Inhabited (α → β) := ⟨λ _ => Inhabited.default⟩
 
 ---
 instance TrivialInhabited (a: α): Inhabited α := ⟨a⟩
